src/bundles_old.lean
@@ -1,0 +1,199 @@
+import tactic
+import .topology
+import .gluing
+import .fiber_product
+
+section fiber_space
+
+variables {E E' B : Type} (π' : E' → B) (φ : E → E')
+
+def res_base (U : set B) :
+  φ ⁻¹' (π' ⁻¹' U) → π' ⁻¹' U :=
+  subtype.map φ (by simp)
+
+@[simp]
+lemma res_base_def (U : set B)
+  (a : E) (ha : a ∈ φ ⁻¹' (π' ⁻¹' U)) :
+  res_base _ _ U ⟨a, ha⟩ = ⟨φ a, ha⟩ := rfl
+
+lemma from_sub_res_image_of_to_sub
+  (U : set B) (V : set E) :
+  from_sub _ ((res_base π' φ U) '' (to_sub _ V)) =
+    (π' ⁻¹' U) ∩ (φ '' V) :=
+begin
+  ext e', simp, split,
+  rintro ⟨e'', he'', ⟨e, he⟩, he12⟩, rw he12 at *,
+  exact ⟨he'', ⟨e, he.1, he.2.2⟩⟩,
+  rintro ⟨he', e, he1, he2⟩, use e', split, exact he', use e,
+  simp [he2], exact ⟨he1, he'⟩,
+end
+
+lemma from_sub_res_preimage_of_to_sub
+  (U : set B) (V : set E') :
+  from_sub _ ((res_base π' φ U) ⁻¹' (to_sub _ V)) = 
+    φ ⁻¹' ((π' ⁻¹' U) ∩ V) :=
+begin
+  unfold from_sub, unfold to_sub, unfold res_base,
+  ext e, simp, split,
+  rintro ⟨x, hx⟩, rw ← hx.2.2, exact ⟨hx.1, hx.2.1⟩,
+  intro h, use e, simp, exact h,
+end
+
+lemma res_base_inj_of_inj
+  (hφ_inj : function.injective φ) (U : set B) : 
+  function.injective (res_base π' φ U) :=
+begin
+  apply subtype.map_injective, exact hφ_inj,
+end
+
+lemma res_base_surj_of_surj
+  (hφ_surj : function.surjective φ) (U : set B) : 
+  function.surjective (res_base π' φ U) :=
+begin
+  rintro ⟨x, hx⟩, obtain ⟨y, hy⟩ := hφ_surj x,
+  use y, simp, rwa hy,
+  simp, exact hy,
+end
+
+lemma res_base_bij_of_bij
+  (hφ_bij : function.bijective φ) (U : set B) : 
+  function.bijective (res_base π' φ U) :=
+begin
+  split,
+    apply res_base_inj_of_inj _ _ hφ_bij.1,
+    apply res_base_surj_of_surj _ _ hφ_bij.2,
+end
+
+
+variables {I : Type} (U : cover I B)
+
+lemma fiber_map_inj_iff_cover_inj :
+  function.injective φ ↔
+  ∀ i, function.injective (res_base π' φ (U i)) :=
+begin
+  split,
+    intros hφ_inj i, apply res_base_inj_of_inj, exact hφ_inj,
+  intros hφ_inj_cover e1 e2 he,
+  obtain ⟨i, hi⟩ := U.hx (π' (φ e1)),
+  specialize @hφ_inj_cover i ⟨e1, hi⟩ ⟨e2, by rwa he at hi⟩,
+  simp at hφ_inj_cover, exact hφ_inj_cover he,
+end
+
+lemma fiber_map_surj_iff_cover_surj :
+  function.surjective φ ↔
+  ∀ i, function.surjective (res_base π' φ (U i)) :=
+begin
+  split,
+    intros hφ_surj i, apply res_base_surj_of_surj, exact hφ_surj,
+  intro hφ_surj_cover, intro e',
+  obtain ⟨i, hi⟩ := U.hx (π' e'),
+  obtain ⟨⟨a, ha⟩, ha'⟩ := hφ_surj_cover i ⟨e', hi⟩,
+  use a, simp at ha', exact ha',
+end
+
+lemma fiber_map_bij_iff_cover_bij :
+  function.bijective φ ↔ 
+  ∀ i, function.bijective (res_base π' φ (U i)) :=
+begin
+  unfold function.bijective,
+  rw forall_and_distrib,
+  rw ← fiber_map_inj_iff_cover_inj,
+  rw ← fiber_map_surj_iff_cover_surj,
+end
+
+section fiber_bundle
+
+open topology
+
+variables [topology B] [topology E] [topology E']
+  {J : Type} (V : open_cover J B)
+
+lemma res_base_cts_of_cts
+  (hπ'_cts : cts π') (hφ_cts : cts φ) (U ∈ opens B) :
+  cts (res_base π' φ U) :=
+  subtype_map_cts hφ_cts
+
+lemma fiber_map_cts_iff_cover_cts
+  (hπ_cts : cts (π' ∘ φ)) (hπ'_cts : cts π') :
+  cts φ ↔
+  ∀ j, cts (res_base π' φ (V j)) :=
+begin
+  split,
+    intros hφ_cts j,
+    apply res_base_cts_of_cts _ _ hπ'_cts hφ_cts _ (V.hopen j),
+  intros hφ_cts_cover,
+  rw cts_iff_ptwise_cts, intros e W hW heW, simp,
+  obtain ⟨j, hj⟩ := V.hx (π' (φ e)),
+  use φ ⁻¹' (π' ⁻¹' (V j) ∩ W),
+  split, -- proof of openness
+    specialize hφ_cts_cover j (to_sub _ W),
+    rw to_sub_open_iff at hφ_cts_cover,
+    specialize hφ_cts_cover ⟨W, hW, rfl⟩,
+    rw from_sub_open_iff at hφ_cts_cover,
+    rwa ← from_sub_res_preimage_of_to_sub,
+    rw ←set.preimage_comp,
+    apply hπ_cts, exact V.hopen j,
+  split, simp, simp, exact ⟨hj, heW⟩,
+end
+
+lemma res_base_open_map_of_open_map
+  (hπ_cts : cts (π' ∘ φ)) (hπ'_cts : cts π')
+  (hφ_open : open_map φ)
+  (U ∈ opens B) :
+  open_map (res_base π' φ U) :=
+begin
+  apply subtype_map_open, exact hφ_open,
+  change ((π' ∘ φ) ⁻¹' U ∈ opens E), apply hπ_cts, exact ‹U ∈ opens B›,
+end
+
+lemma fiber_map_open_map_iff_res_open_map
+  (hπ_cts : cts (π' ∘ φ)) (hπ'_cts : cts π') :
+  open_map φ ↔
+  ∀ j, open_map (res_base π' φ (V j)) :=
+begin
+  split,
+    intros hφ_open j,
+    apply res_base_open_map_of_open_map _ _ hπ_cts hπ'_cts hφ_open _ (V.hopen j),
+  intros hφ_open_map W hW,
+  rw subset_open_iff_open_cover (pullback_open_cover π' hπ'_cts V),
+  intro j, change π' ⁻¹' (V j) ∩ φ '' W ∈ opens E',
+  specialize hφ_open_map j (to_sub _ W),
+  rw to_sub_open_iff at hφ_open_map,
+  specialize hφ_open_map ⟨W, hW, rfl⟩,
+  rw from_sub_open_iff at hφ_open_map,
+  rwa ← from_sub_res_image_of_to_sub,
+  apply hπ'_cts, exact V.hopen j,
+end
+
+lemma res_base_homeo_of_homeo
+  (hπ_cts : cts (π' ∘ φ)) (hπ'_cts : cts π')
+  (hφ_homeo : homeo φ)
+  (U ∈ opens B) :
+  homeo (res_base π' φ U) :=
+begin
+  rw homeo_iff at *,
+  split,
+    exact res_base_cts_of_cts _ _ hπ'_cts hφ_homeo.1 U ‹U ∈ opens B›,
+  split,
+    exact res_base_bij_of_bij _ _ hφ_homeo.2.1 U,
+    exact res_base_open_map_of_open_map _ _ hπ_cts hπ'_cts hφ_homeo.2.2 U ‹U ∈ opens B›,
+end
+
+lemma fiber_map_homeo_iff_res_homeo
+  (hπ_cts : cts (π' ∘ φ)) (hπ'_cts : cts π') :
+  homeo φ ↔
+  ∀ j, homeo (res_base π' φ (V j)) :=
+begin
+  split, intros hφ_homeo j,
+    exact res_base_homeo_of_homeo _ _ hπ_cts hπ'_cts hφ_homeo (V j) (V.hopen j),
+  intro hφ_homeo,
+  rw [homeo_iff,
+      fiber_map_cts_iff_cover_cts _ _ V hπ_cts hπ'_cts,
+      fiber_map_bij_iff_cover_bij _ _ V.to_cover,
+      fiber_map_open_map_iff_res_open_map _ _ V hπ_cts hπ'_cts,
+      ← forall_and_distrib, ← forall_and_distrib],
+  intro j, specialize hφ_homeo j, rwa homeo_iff at hφ_homeo,
+end
+
+end fiber_bundle
+end fiber_space
